MPoly_PM.thy
@@ -1,0 +1,796 @@
+section \<open>Multivariate Polynomials with Power-Products Represented by Polynomial Mappings\<close>
+
+theory MPoly_PM
+  imports Poly_Utils
+begin
+
+text \<open>Many notions introduced in this theory for type @{typ "('n \<Rightarrow>\<^sub>0 'a) \<Rightarrow>\<^sub>0 'b"} closely resemble
+  those introduced in @{theory MPoly_Type} for type @{typ "'a mpoly"}.\<close>
+
+lemma monomial_single_power:
+  "(monomial c (Poly_Mapping.single x k)) ^ n = monomial (c ^ n) (Poly_Mapping.single x (k * n))"
+proof -
+  have eq: "(\<Sum>i = 0..<n. Poly_Mapping.single x k) = Poly_Mapping.single x (k * n)"
+    by (induct n, simp_all add: add.commute single_add)
+  show ?thesis by (simp add: monomial_power eq)
+qed
+
+lemma deg_pm_single: "deg_pm (Poly_Mapping.single x k) = k"
+proof -
+  have "keys (Poly_Mapping.single x k) \<subseteq> {x}" by simp
+  moreover have "finite {x}" by simp
+  ultimately have "deg_pm (Poly_Mapping.single x k) = (\<Sum>y\<in>{x}. lookup (Poly_Mapping.single x k) y)"
+    by (rule deg_pm_superset)
+  also have "... = k" by simp
+  finally show ?thesis .
+qed
+
+subsection \<open>Order relation on polynomial mappings\<close>
+
+definition le_pm :: "('a \<Rightarrow>\<^sub>0 'b) \<Rightarrow> ('a \<Rightarrow>\<^sub>0 'b::{ord,zero}) \<Rightarrow> bool" (infixl "\<unlhd>" 50)
+  where "le_pm s t \<longleftrightarrow> (lookup s \<le> lookup t)"
+
+lemma le_pmI:
+  assumes "\<And>x. lookup s x \<le> lookup t x"
+  shows "s \<unlhd> t"
+  unfolding le_pm_def le_fun_def using assms ..
+
+lemma le_pmD:
+  assumes "s \<unlhd> t"
+  shows "lookup s x \<le> lookup t x"
+  using assms unfolding le_pm_def le_fun_def ..
+
+lemma adds_pmI:
+  assumes "s \<unlhd> t"
+  shows "s adds (t::'a \<Rightarrow>\<^sub>0 'b::add_linorder)"
+  using assms by (simp add: le_pm_def, intro adds_poly_mappingI)
+
+lemma adds_pm: "s adds t \<longleftrightarrow> s \<unlhd> t"
+  for s t::"'a \<Rightarrow>\<^sub>0 'b::add_linorder_min"
+  by (simp add: adds_poly_mapping le_pm_def)
+
+subsection \<open>Degree\<close>
+
+definition poly_deg :: "(('n \<Rightarrow>\<^sub>0 'a::add_linorder) \<Rightarrow>\<^sub>0 'b::zero) \<Rightarrow> 'a" where
+  "poly_deg p = (if keys p = {} then 0 else Max (deg_pm ` keys p))"
+
+definition maxdeg :: "(('n \<Rightarrow>\<^sub>0 'a::add_linorder) \<Rightarrow>\<^sub>0 'b::zero) set \<Rightarrow> 'a" where
+  "maxdeg A = Max (poly_deg ` A)"
+  
+definition mindeg :: "(('n \<Rightarrow>\<^sub>0 'a::add_linorder) \<Rightarrow>\<^sub>0 'b::zero) set \<Rightarrow> 'a" where
+  "mindeg A = Min (poly_deg ` A)"
+
+lemma poly_deg_monomial: "poly_deg (monomial c t) = (if c = 0 then 0 else deg_pm t)"
+  by (simp add: poly_deg_def)
+
+lemma poly_deg_monomial_zero [simp]: "poly_deg (monomial c 0) = 0"
+  by (simp add: poly_deg_monomial)
+
+lemma poly_deg_zero [simp]: "poly_deg 0 = 0"
+  by (simp only: single_zero[of 0, symmetric] poly_deg_monomial_zero)
+
+lemma poly_deg_one [simp]: "poly_deg 1 = 0"
+  by (simp only: single_one[symmetric] poly_deg_monomial_zero)
+
+lemma poly_deg_max_keys:
+  assumes "t \<in> keys p"
+  shows "deg_pm t \<le> poly_deg p"
+  unfolding poly_deg_def using finite_keys assms by auto
+
+lemma poly_deg_leI:
+  assumes "\<And>t. t \<in> keys p \<Longrightarrow> deg_pm t \<le> (d::'a::add_linorder_min)"
+  shows "poly_deg p \<le> d"
+  unfolding poly_deg_def using finite_keys assms by auto
+
+lemma poly_deg_zero_imp_monomial:
+  assumes "poly_deg p = (0::'a::add_linorder_min)"
+  shows "monomial (lookup p 0) 0 = p"
+proof (rule keys_subset_singleton_imp_monomial, rule)
+  fix t
+  assume "t \<in> keys p"
+  have "t = 0"
+  proof (rule ccontr)
+    assume "t \<noteq> 0"
+    hence "deg_pm t \<noteq> 0" by simp
+    hence "0 < deg_pm t" using not_gr_zero by blast
+    also from \<open>t \<in> keys p\<close> have "... \<le> poly_deg p" by (rule poly_deg_max_keys)
+    finally have "poly_deg p \<noteq> 0" by simp
+    from this assms show False ..
+  qed
+  thus "t \<in> {0}" by simp
+qed
+
+lemma poly_deg_plus_le:
+  "poly_deg (p + q) \<le> max (poly_deg p) (poly_deg (q::(_ \<Rightarrow>\<^sub>0 'a::add_linorder_min) \<Rightarrow>\<^sub>0 _))"
+proof (rule poly_deg_leI)
+  fix t
+  assume "t \<in> keys (p + q)"
+  also have "... \<subseteq> keys p \<union> keys q" by (fact keys_add_subset)
+  finally show "deg_pm t \<le> max (poly_deg p) (poly_deg q)"
+  proof
+    assume "t \<in> keys p"
+    hence "deg_pm t \<le> poly_deg p" by (rule poly_deg_max_keys)
+    thus ?thesis by (simp add: le_max_iff_disj)
+  next
+    assume "t \<in> keys q"
+    hence "deg_pm t \<le> poly_deg q" by (rule poly_deg_max_keys)
+    thus ?thesis by (simp add: le_max_iff_disj)
+  qed
+qed
+
+lemma poly_deg_uminus [simp]: "poly_deg (-p) = poly_deg p"
+  by (simp add: poly_deg_def keys_uminus)
+
+lemma poly_deg_minus_le:
+  "poly_deg (p - q) \<le> max (poly_deg p) (poly_deg (q::(_ \<Rightarrow>\<^sub>0 'a::add_linorder_min) \<Rightarrow>\<^sub>0 _))"
+proof (rule poly_deg_leI)
+  fix t
+  assume "t \<in> keys (p - q)"
+  also have "... \<subseteq> keys p \<union> keys q" by (fact keys_minus)
+  finally show "deg_pm t \<le> max (poly_deg p) (poly_deg q)"
+  proof
+    assume "t \<in> keys p"
+    hence "deg_pm t \<le> poly_deg p" by (rule poly_deg_max_keys)
+    thus ?thesis by (simp add: le_max_iff_disj)
+  next
+    assume "t \<in> keys q"
+    hence "deg_pm t \<le> poly_deg q" by (rule poly_deg_max_keys)
+    thus ?thesis by (simp add: le_max_iff_disj)
+  qed
+qed
+
+lemma poly_deg_times_le:
+  "poly_deg (p * q) \<le> poly_deg p + poly_deg (q::(_ \<Rightarrow>\<^sub>0 'a::add_linorder_min) \<Rightarrow>\<^sub>0 _)"
+proof (rule poly_deg_leI)
+  fix t
+  assume "t \<in> keys (p * q)"
+  then obtain u v where "u \<in> keys p" and "v \<in> keys q" and "t = u + v" by (rule in_keys_timesE)
+  from \<open>u \<in> keys p\<close> have "deg_pm u \<le> poly_deg p" by (rule poly_deg_max_keys)
+  moreover from \<open>v \<in> keys q\<close> have "deg_pm v \<le> poly_deg q" by (rule poly_deg_max_keys)
+  ultimately show "deg_pm t \<le> poly_deg p + poly_deg q" by (simp add: \<open>t = u + v\<close> deg_pm_plus add_mono)
+qed
+
+corollary poly_deg_monom_mult_le:
+  "poly_deg (monom_mult c (t::_ \<Rightarrow>\<^sub>0 'a::add_linorder_min) p) \<le> deg_pm t + poly_deg p"
+proof -
+  have "poly_deg (monom_mult c t p) \<le> poly_deg (monomial c t) + poly_deg p"
+    by (simp only: times_monomial_left[symmetric] poly_deg_times_le)
+  also have "... \<le> deg_pm t + poly_deg p" by (simp add: poly_deg_monomial)
+  finally show ?thesis .
+qed
+
+lemma poly_deg_monom_mult:
+  assumes "c \<noteq> 0" and "p \<noteq> (0::(_ \<Rightarrow>\<^sub>0 'a::add_linorder_min) \<Rightarrow>\<^sub>0 'b::semiring_no_zero_divisors)"
+  shows "poly_deg (monom_mult c t p) = deg_pm t + poly_deg p"
+proof (rule order.antisym, fact poly_deg_monom_mult_le)
+  from assms(2) have "keys p \<noteq> {}" by simp
+  then obtain s where "s \<in> keys p" and "poly_deg p = deg_pm s" unfolding poly_deg_def
+    by (metis (mono_tags, lifting) finite_keys Max_in finite_imageI image_iff image_is_empty)
+  have "deg_pm t + poly_deg p = deg_pm (t + s)" by (simp add: \<open>poly_deg p = deg_pm s\<close> deg_pm_plus)
+  also have "... \<le> poly_deg (monom_mult c t p)"
+  proof (rule poly_deg_max_keys)
+    from \<open>s \<in> keys p\<close> show "t + s \<in> keys (monom_mult c t p)"
+      unfolding keys_monom_mult[OF assms(1)] by fastforce
+  qed
+  finally show "deg_pm t + poly_deg p \<le> poly_deg (monom_mult c t p)" .
+qed
+
+lemma poly_deg_sum_le: "((poly_deg (sum f A))::'a::add_linorder_min) \<le> Max (poly_deg ` f ` A)"
+proof (cases "finite A")
+  case True
+  thus ?thesis
+  proof (induct A)
+    case empty
+    show ?case by simp
+  next
+    case (insert a A)
+    show ?case
+    proof (cases "A = {}")
+      case True
+      thus ?thesis by simp
+    next
+      case False
+      have "poly_deg (sum f (insert a A)) \<le> max (poly_deg (f a)) (poly_deg (sum f A))"
+        by (simp only: comm_monoid_add_class.sum.insert[OF insert(1) insert(2)] poly_deg_plus_le)
+      also have "... \<le> max (poly_deg (f a)) (Max (poly_deg ` f ` A))"
+        using insert(3) max.mono by blast
+      also have "... = (Max (poly_deg ` f ` (insert a A)))" using False by (simp add: insert(1))
+      finally show ?thesis .
+    qed
+  qed
+next
+  case False
+  thus ?thesis by simp
+qed
+
+lemma poly_deg_prod_le: "((poly_deg (prod f A))::'a::add_linorder_min) \<le> (\<Sum>a\<in>A. poly_deg (f a))"
+proof (cases "finite A")
+  case True
+  thus ?thesis
+  proof (induct A)
+    case empty
+    show ?case by simp
+  next
+    case (insert a A)
+    have "poly_deg (prod f (insert a A)) \<le> (poly_deg (f a)) + (poly_deg (prod f A))"
+      by (simp only: comm_monoid_mult_class.prod.insert[OF insert(1) insert(2)] poly_deg_times_le)
+    also have "... \<le> (poly_deg (f a)) + (\<Sum>a\<in>A. poly_deg (f a))"
+      using insert(3) add_le_cancel_left by blast
+    also have "... = (\<Sum>a\<in>insert a A. poly_deg (f a))" by (simp add: insert(1) insert(2))
+    finally show ?case .
+  qed
+next
+  case False
+  thus ?thesis by simp
+qed
+
+lemma maxdeg_max:
+  assumes "finite A" and "p \<in> A"
+  shows "poly_deg p \<le> maxdeg A"
+  unfolding maxdeg_def using assms by auto
+
+lemma mindeg_min:
+  assumes "finite A" and "p \<in> A"
+  shows "mindeg A \<le> poly_deg p"
+  unfolding mindeg_def using assms by auto
+
+subsection \<open>Indeterminates\<close>
+
+definition indets :: "(('n \<Rightarrow>\<^sub>0 'a::zero) \<Rightarrow>\<^sub>0 'b::zero) \<Rightarrow> 'n set"
+  where "indets p = UNION (keys p) keys"
+
+lemma in_indetsI:
+  assumes "x \<in> keys t" and "t \<in> keys p"
+  shows "x \<in> indets p"
+  using assms by (auto simp add: indets_def)
+
+lemma in_indetsE:
+  assumes "x \<in> indets p"
+  obtains t where "t \<in> keys p" and "x \<in> keys t"
+  using assms by (auto simp add: indets_def)
+
+lemma indets_empty_imp_monomial:
+  assumes "indets p = {}"
+  shows "monomial (lookup p 0) 0 = p"
+proof (rule keys_subset_singleton_imp_monomial, rule)
+  fix t
+  assume "t \<in> keys p"
+  have "t = 0"
+  proof (rule ccontr)
+    assume "t \<noteq> 0"
+    hence "keys t \<noteq> {}" by simp
+    then obtain x where "x \<in> keys t" by blast
+    from this \<open>t \<in> keys p\<close> have "x \<in> indets p" by (rule in_indetsI)
+    with assms show False by simp
+  qed
+  thus "t \<in> {0}" by simp
+qed
+
+lemma finite_indets: "finite (indets p)"
+  by (simp only: indets_def, rule finite_UN_I, (rule finite_keys)+)
+
+lemma indets_zero [simp]: "indets 0 = {}"
+  by (simp add: indets_def)
+
+lemma indets_one [simp]: "indets 1 = {}"
+  by (simp add: indets_def)
+
+lemma indets_monomial_single_subset: "indets (monomial c (Poly_Mapping.single v k)) \<subseteq> {v}"
+proof
+  fix x assume "x \<in> indets (monomial c (Poly_Mapping.single v k))"
+  then have "x = v" unfolding indets_def
+    by (metis UN_E lookup_eq_zero_in_keys_contradict lookup_single_not_eq)
+  thus "x \<in> {v}" by simp
+qed
+
+lemma indets_monomial_single:
+  assumes "c \<noteq> 0" and "k \<noteq> 0"
+  shows "indets (monomial c (Poly_Mapping.single v k)) = {v}"
+proof (rule, fact indets_monomial_single_subset, simp)
+  from assms show "v \<in> indets (monomial c (monomial k v))" by (simp add: indets_def)
+qed
+
+lemma indets_monomial:
+  assumes "c \<noteq> 0"
+  shows "indets (monomial c t) = keys t"
+proof (rule antisym; rule subsetI)
+  fix x
+  assume "x \<in> indets (monomial c t)"
+  then have "lookup t x \<noteq> 0" unfolding indets_def
+    by (metis UN_E lookup_eq_zero_in_keys_contradict lookup_single_not_eq)
+  thus "x \<in> keys t" by (meson lookup_not_eq_zero_eq_in_keys)
+next
+  fix x
+  assume "x \<in> keys t"
+  then have "lookup t x \<noteq> 0" by (meson lookup_not_eq_zero_eq_in_keys)
+  thus "x \<in> indets (monomial c t)" unfolding indets_def using assms
+    by (metis UN_iff lookup_not_eq_zero_eq_in_keys lookup_single_eq)
+qed
+
+lemma indets_monomial_subset: "indets (monomial c t) \<subseteq> keys t"
+  by (cases "c = 0", simp_all add: indets_def)
+
+lemma indets_monomial_zero [simp]: "indets (monomial c 0) = {}"
+  by (simp add: indets_def)
+
+lemma indets_plus_subset: "indets (p + q) \<subseteq> indets p \<union> indets q"
+proof
+  fix x
+  assume "x \<in> indets (p + q)"
+  then obtain t where "x \<in> keys t" and "t \<in> keys (p + q)" by (metis UN_E indets_def)
+  hence "t \<in> keys p \<union> keys q" by (metis keys_add_subset subsetCE)
+  thus "x \<in> indets p \<union> indets q" using indets_def \<open>x \<in> keys t\<close> by fastforce
+qed
+
+lemma indets_uminus [simp]: "indets (-p) = indets p"
+  by (simp add: indets_def keys_uminus)
+
+lemma indets_minus_subset: "indets (p - q) \<subseteq> indets p \<union> indets q"
+proof
+  fix x
+  assume "x \<in> indets (p - q)"
+  then obtain t where "x \<in> keys t" and "t \<in> keys (p - q)" by (metis UN_E indets_def)
+  hence "t \<in> keys p \<union> keys q" by (metis keys_minus subsetCE)
+  thus "x \<in> indets p \<union> indets q" using indets_def \<open>x \<in> keys t\<close> by fastforce
+qed
+
+lemma indets_times_subset: "indets (p * q) \<subseteq> indets p \<union> indets q"
+proof
+  fix x
+  assume "x \<in> indets (p * q)"
+  then obtain t where "t \<in> keys (p * q)" and "x \<in> keys t" unfolding indets_def by blast
+  from this(1) obtain u v where "u \<in> keys p" "v \<in> keys q" and "t = u + v" by (rule in_keys_timesE)
+  hence "x \<in> keys u \<union> keys v" by (metis \<open>x \<in> keys t\<close> keys_add_subset subsetCE)
+  thus "x \<in> indets p \<union> indets q" unfolding indets_def using \<open>u \<in> keys p\<close> \<open>v \<in> keys q\<close> by blast
+qed
+
+corollary indets_monom_mult_subset: "indets (monom_mult c t p) \<subseteq> keys t \<union> indets p"
+proof -
+  have "indets (monom_mult c t p) \<subseteq> indets (monomial c t) \<union> indets p"
+    by (simp only: times_monomial_left[symmetric] indets_times_subset)
+  also have "... \<subseteq> keys t \<union> indets p" using indets_monomial_subset[of t c] by blast
+  finally show ?thesis .
+qed
+
+lemma indets_monom_mult:
+  assumes "c \<noteq> 0" and "p \<noteq> (0::('n \<Rightarrow>\<^sub>0 'a::{comm_powerprod,ninv_comm_monoid_add}) \<Rightarrow>\<^sub>0 'b::semiring_no_zero_divisors)"
+  shows "indets (monom_mult c t p) = keys t \<union> indets p"
+proof (rule, fact indets_monom_mult_subset, rule)
+  fix x
+  assume "x \<in> keys t \<union> indets p"
+  thus "x \<in> indets (monom_mult c t p)"
+  proof
+    assume "x \<in> keys t"
+    from assms(2) have "keys p \<noteq> {}" by simp
+    then obtain s where "s \<in> keys p" by blast
+    hence "t + s \<in> (+) t ` keys p" by fastforce
+    also from assms(1) have "... = keys (monom_mult c t p)" by (simp add: keys_monom_mult)
+    finally have "t + s \<in> keys (monom_mult c t p)" .
+    show ?thesis
+    proof (rule in_indetsI)
+      from \<open>x \<in> keys t\<close> show "x \<in> keys (t + s)" by (simp add: keys_plus_ninv_comm_monoid_add)
+    qed fact
+  next
+    assume "x \<in> indets p"
+    then obtain s where "s \<in> keys p" and "x \<in> keys s" by (rule in_indetsE)
+    from this(1) have "t + s \<in> (+) t ` keys p" by fastforce
+    also from assms(1) have "... = keys (monom_mult c t p)" by (simp add: keys_monom_mult)
+    finally have "t + s \<in> keys (monom_mult c t p)" .
+    show ?thesis
+    proof (rule in_indetsI)
+      from \<open>x \<in> keys s\<close> show "x \<in> keys (t + s)" by (simp add: keys_plus_ninv_comm_monoid_add)
+    qed fact
+  qed
+qed
+
+lemma indets_sum_subset: "indets (sum f A) \<subseteq> (\<Union>a\<in>A. indets (f a))"
+proof (cases "finite A")
+  case True
+  thus ?thesis
+  proof (induct A)
+    case empty
+    show ?case by simp
+  next
+    case (insert a A)
+    have "indets (sum f (insert a A)) \<subseteq> indets (f a) \<union> indets (sum f A)"
+      by (simp only: comm_monoid_add_class.sum.insert[OF insert(1) insert(2)] indets_plus_subset)
+    also have "... \<subseteq> indets (f a) \<union> (\<Union>a\<in>A. indets (f a))" using insert(3) by blast
+    also have "... = (\<Union>a\<in>insert a A. indets (f a))" by simp
+    finally show ?case .
+  qed
+next
+  case False
+  thus ?thesis by simp
+qed
+
+lemma indets_prod_subset: "indets (prod f A) \<subseteq> (\<Union>a\<in>A. indets (f a))"
+proof (cases "finite A")
+  case True
+  thus ?thesis
+  proof (induct A)
+    case empty
+    show ?case by simp
+  next
+    case (insert a A)
+    have "indets (prod f (insert a A)) \<subseteq> indets (f a) \<union> indets (prod f A)"
+      by (simp only: comm_monoid_mult_class.prod.insert[OF insert(1) insert(2)] indets_times_subset)
+    also have "... \<subseteq> indets (f a) \<union> (\<Union>a\<in>A. indets (f a))" using insert(3) by blast
+    also have "... = (\<Union>a\<in>insert a A. indets (f a))" by simp
+    finally show ?case .
+  qed
+next
+  case False
+  thus ?thesis by simp
+qed
+
+lemma indets_power_subset: "indets (p ^ n) \<subseteq> indets (p::('n \<Rightarrow>\<^sub>0 nat) \<Rightarrow>\<^sub>0 'b::comm_semiring_1)"
+proof -
+  have "p ^ n = (\<Prod>i=0..<n. p)" by (simp add: prod_constant)
+  also have "indets ... \<subseteq> (\<Union>i\<in>{0..<n}. indets p)" by (fact indets_prod_subset)
+  also have "... \<subseteq> indets p" by simp
+  finally show ?thesis .
+qed
+
+lemma indets_empty_iff_poly_deg_zero: "indets p = {} \<longleftrightarrow> poly_deg p = (0::'a::add_linorder_min)"
+proof
+  assume "indets p = {}"
+  hence "monomial (lookup p 0) 0 = p" by (rule indets_empty_imp_monomial)
+  moreover have "poly_deg (monomial (lookup p 0) 0) = 0" by simp
+  ultimately show "poly_deg p = 0" by metis
+next
+  assume "poly_deg p = 0"
+  hence "monomial (lookup p 0) 0 = p" by (rule poly_deg_zero_imp_monomial)
+  moreover have "indets (monomial (lookup p 0) 0) = {}" by simp
+  ultimately show "indets p = {}" by metis
+qed
+
+subsection \<open>Substitution Homomorphisms\<close>
+
+text \<open>The substitution homomorphisms defined here are more general than @{const insertion} etc., since
+  they replace indeterminates by @{emph \<open>polynomials\<close>} rather than coefficients, and therefore
+  construct new polynomials.\<close>
+
+definition subst_pp :: "('n \<Rightarrow> (('n \<Rightarrow>\<^sub>0 nat) \<Rightarrow>\<^sub>0 'a)) \<Rightarrow> ('n \<Rightarrow>\<^sub>0 nat) \<Rightarrow> (('n \<Rightarrow>\<^sub>0 nat) \<Rightarrow>\<^sub>0 'a::comm_semiring_1)"
+  where "subst_pp f t = (\<Prod>x\<in>keys t. (f x) ^ (lookup t x))"
+
+definition poly_subst :: "('n \<Rightarrow> (('n \<Rightarrow>\<^sub>0 nat) \<Rightarrow>\<^sub>0 'a)) \<Rightarrow> (('n \<Rightarrow>\<^sub>0 nat) \<Rightarrow>\<^sub>0 'a) \<Rightarrow> (('n \<Rightarrow>\<^sub>0 nat) \<Rightarrow>\<^sub>0 'a::comm_semiring_1)"
+  where "poly_subst f p = (\<Sum>t\<in>keys p. monom_mult (lookup p t) 0 (subst_pp f t))"
+
+lemma subst_pp_alt: "subst_pp f t = (\<Prod>x. (f x) ^ (lookup t x))"
+proof -
+  from finite_keys have "subst_pp f t = (\<Prod>x. if x \<in> keys t then (f x) ^ (lookup t x) else 1)"
+    unfolding subst_pp_def by (rule Prod_any.conditionalize)
+  also have "... = (\<Prod>x. (f x) ^ (lookup t x))" by (rule Prod_any.cong, simp)
+  finally show ?thesis .
+qed
+
+lemma subst_pp_zero [simp]: "subst_pp f 0 = 1"
+  by (simp add: subst_pp_def)
+
+lemma subst_pp_trivial_not_zero:
+  assumes "t \<noteq> 0"
+  shows "subst_pp (\<lambda>_. 0) t = (0::(('n \<Rightarrow>\<^sub>0 nat) \<Rightarrow>\<^sub>0 'b::comm_semiring_1))"
+  unfolding subst_pp_def using finite_keys
+proof (rule prod_zero)
+  from assms have "keys t \<noteq> {}" by simp
+  then obtain x where "x \<in> keys t" by blast
+  thus "\<exists>x\<in>keys t. 0 ^ lookup t x = (0::(('n \<Rightarrow>\<^sub>0 nat) \<Rightarrow>\<^sub>0 'b))"
+  proof
+    from \<open>x \<in> keys t\<close> have "0 < lookup t x" by (simp add: in_keys_iff)
+    thus "0 ^ lookup t x = (0::(('n \<Rightarrow>\<^sub>0 nat) \<Rightarrow>\<^sub>0 'b))" by (rule Power.semiring_1_class.zero_power)
+  qed
+qed
+
+corollary subst_pp_trivial: "subst_pp (\<lambda>_. 0) t = (if t = 0 then 1 else 0)"
+  by (simp split: if_split add: subst_pp_trivial_not_zero)
+
+lemma power_lookup_not_one_subset_keys: "{x. f x ^ (lookup t x) \<noteq> 1} \<subseteq> keys t"
+proof (rule, simp)
+  fix x
+  assume "f x ^ (lookup t x) \<noteq> 1"
+  thus "x \<in> keys t" unfolding in_keys_iff by (metis power_0)
+qed
+
+corollary finite_power_lookup_not_one: "finite {x. f x ^ (lookup t x) \<noteq> 1}"
+  by (rule finite_subset, fact power_lookup_not_one_subset_keys, fact finite_keys)
+
+lemma subst_pp_plus: "subst_pp f (s + t) = subst_pp f s * subst_pp f t"
+  by (simp add: subst_pp_alt lookup_add power_add, rule Prod_any.distrib, (fact finite_power_lookup_not_one)+)
+
+lemma subst_pp_id:
+  assumes "\<And>x. x \<in> keys t \<Longrightarrow> f x = monomial 1 (Poly_Mapping.single x 1)"
+  shows "subst_pp f t = monomial 1 t"
+proof -
+  have "subst_pp f t = (\<Prod>x\<in>keys t. monomial 1 (Poly_Mapping.single x (lookup t x)))"
+  proof (simp only: subst_pp_def, rule prod.cong, fact refl)
+    fix x
+    assume "x \<in> keys t"
+    thus "f x ^ lookup t x = monomial 1 (Poly_Mapping.single x (lookup t x))"
+      by (simp add: assms monomial_single_power)
+  qed
+  also have "... = monomial 1 t" by (simp add: monomial_prod[symmetric] poly_mapping_sum_monomials)
+  finally show ?thesis .
+qed
+
+lemma in_indets_subst_ppE:
+  assumes "x \<in> indets (subst_pp f t)"
+  obtains y where "y \<in> keys t" and "x \<in> indets (f y)"
+proof -
+  note assms
+  also have "indets (subst_pp f t) \<subseteq> (\<Union>y\<in>keys t. indets ((f y) ^ (lookup t y)))" unfolding subst_pp_def
+    by (rule indets_prod_subset)
+  finally obtain y where "y \<in> keys t" and "x \<in> indets ((f y) ^ (lookup t y))" ..
+  note this(2)
+  also have "indets ((f y) ^ (lookup t y)) \<subseteq> indets (f y)" by (rule indets_power_subset)
+  finally have "x \<in> indets (f y)" .
+  with \<open>y \<in> keys t\<close> show ?thesis ..
+qed
+
+lemma poly_deg_subst_pp_eq_zeroI:
+  assumes "\<And>x. x \<in> keys t \<Longrightarrow> poly_deg (f x) = 0"
+  shows "poly_deg (subst_pp f (t::'n \<Rightarrow>\<^sub>0 nat)) = 0"
+proof -
+  have "poly_deg (subst_pp f t) \<le> (\<Sum>x\<in>keys t. poly_deg ((f x) ^ (lookup t x)))"
+    unfolding subst_pp_def by (fact poly_deg_prod_le)
+  also have "... = 0"
+  proof (rule sum.neutral, rule)
+    fix x
+    assume "x \<in> keys t"
+    hence "poly_deg (f x) = 0" by (rule assms)
+    have "f x ^ lookup t x = (\<Prod>i=0..<lookup t x. f x)" by (simp add: prod_constant)
+    also have "poly_deg ... \<le> (\<Sum>i=0..<lookup t x. poly_deg (f x))" by (rule poly_deg_prod_le)
+    also have "... = 0" by (simp add: \<open>poly_deg (f x) = 0\<close>)
+    finally show "poly_deg (f x ^ lookup t x) = 0" by simp
+  qed
+  finally show ?thesis by simp
+qed
+
+lemma poly_deg_subst_pp_le:
+  assumes "\<And>x. x \<in> keys t \<Longrightarrow> poly_deg (f x) \<le> 1"
+  shows "poly_deg (subst_pp f (t::'n \<Rightarrow>\<^sub>0 nat)) \<le> deg_pm t"
+proof -
+  have "poly_deg (subst_pp f t) \<le> (\<Sum>x\<in>keys t. poly_deg ((f x) ^ (lookup t x)))"
+    unfolding subst_pp_def by (fact poly_deg_prod_le)
+  also have "... \<le> (\<Sum>x\<in>keys t. lookup t x)"
+  proof (rule sum_mono)
+    fix x
+    assume "x \<in> keys t"
+    hence "poly_deg (f x) \<le> 1" by (rule assms)
+    have "f x ^ lookup t x = (\<Prod>i=0..<lookup t x. f x)" by (simp add: prod_constant)
+    also have "poly_deg ... \<le> (\<Sum>i=0..<lookup t x. poly_deg (f x))" by (rule poly_deg_prod_le)
+    also from \<open>poly_deg (f x) \<le> 1\<close> have "... \<le> (\<Sum>i=0..<lookup t x. 1)" by (rule sum_mono)
+    finally show "poly_deg (f x ^ lookup t x) \<le> lookup t x" by simp
+  qed
+  also have "... = deg_pm t" by (rule deg_pm_superset[symmetric], fact subset_refl, fact finite_keys)
+  finally show ?thesis by simp
+qed
+
+lemma poly_subst_alt: "poly_subst f p = (\<Sum>t. monom_mult (lookup p t) 0 (subst_pp f t))"
+proof -
+  from finite_keys have "poly_subst f p = (\<Sum>t. if t \<in> keys p then monom_mult (lookup p t) 0 (subst_pp f t) else 0)"
+    unfolding poly_subst_def by (rule Sum_any.conditionalize)
+  also have "... = (\<Sum>t. monom_mult (lookup p t) 0 (subst_pp f t))"
+    by (rule Sum_any.cong, simp add: monom_mult_left0)
+  finally show ?thesis .
+qed
+
+lemma poly_subst_trivial [simp]: "poly_subst (\<lambda>_. 0) p = monomial (lookup p 0) 0"
+  apply (simp add: poly_subst_def subst_pp_trivial if_distrib)
+  apply (simp add: monom_mult_right0 cong: if_cong)
+  apply (metis mult.right_neutral times_monomial_left)
+  done
+
+lemma poly_subst_zero [simp]: "poly_subst f 0 = 0"
+  by (simp add: poly_subst_def)
+
+lemma monom_mult_lookup_not_zero_subset_keys: "{t. monom_mult (lookup p t) 0 (subst_pp f t) \<noteq> 0} \<subseteq> keys p"
+proof (rule, simp)
+  fix t
+  assume "monom_mult (lookup p t) 0 (subst_pp f t) \<noteq> 0"
+  thus "t \<in> keys p" unfolding in_keys_iff by (metis monom_mult_left0)
+qed
+
+corollary finite_monom_mult_lookup_not_zero: "finite {t. monom_mult (lookup p t) 0 (subst_pp f t) \<noteq> 0}"
+  by (rule finite_subset, fact monom_mult_lookup_not_zero_subset_keys, fact finite_keys)
+
+lemma poly_subst_plus: "poly_subst f (p + q) = poly_subst f p + poly_subst f q"
+  by (simp add: poly_subst_alt lookup_add monom_mult_dist_left, rule Sum_any.distrib,
+      (fact finite_monom_mult_lookup_not_zero)+)
+
+lemma poly_subst_uminus: "poly_subst f (-p) = - poly_subst f (p::('n \<Rightarrow>\<^sub>0 nat) \<Rightarrow>\<^sub>0 'b::comm_ring_1)"
+  by (simp add: poly_subst_def keys_uminus monom_mult_uminus_left sum_negf)
+
+lemma poly_subst_minus: "poly_subst f (p - q) = poly_subst f p - poly_subst f (q::('n \<Rightarrow>\<^sub>0 nat) \<Rightarrow>\<^sub>0 'b::comm_ring_1)"
+proof -
+  have "poly_subst f (p + (-q)) = poly_subst f p + poly_subst f (-q)" by (fact poly_subst_plus)
+  thus ?thesis by (simp add: poly_subst_uminus)
+qed
+
+lemma poly_subst_monomial: "poly_subst f (monomial c t) = monom_mult c 0 (subst_pp f t)"
+  by (simp add: poly_subst_def lookup_single monom_mult_left0)
+
+corollary poly_subst_one [simp]: "poly_subst f 1 = 1"
+  by (simp add: single_one[symmetric] poly_subst_monomial monom_mult_monomial del: single_one)
+
+lemma poly_subst_times: "poly_subst f (p * q) = poly_subst f p * poly_subst f q"
+proof -
+  have bij: "bij (\<lambda>(l, n, m). (m, l, n))"
+    by (auto intro!: bijI injI simp add: image_def)
+  let ?P = "keys p"
+  let ?Q = "keys q"
+  let ?PQ = "{s + t | s t. lookup p s \<noteq> 0 \<and> lookup q t \<noteq> 0}"
+  have fin_PQ: "finite ?PQ"
+    by (rule finite_not_eq_zero_sumI, simp_all)
+  have fin_1: "finite {l. lookup p l * (\<Sum>qa. lookup q qa when t = l + qa) \<noteq> 0}" for t
+  proof (rule finite_subset)
+    show "{l. lookup p l * (\<Sum>qa. lookup q qa when t = l + qa) \<noteq> 0} \<subseteq> keys p"
+      by (rule, auto simp add: in_keys_iff simp del: lookup_not_eq_zero_eq_in_keys)
+  qed (fact finite_keys)
+  have fin_2: "finite {v. (lookup q v when t = u + v) \<noteq> 0}" for t u
+  proof (rule finite_subset)
+    show "{v. (lookup q v when t = u + v) \<noteq> 0} \<subseteq> keys q"
+      by (rule, auto simp add: in_keys_iff simp del: lookup_not_eq_zero_eq_in_keys)
+  qed (fact finite_keys)
+  have fin_3: "finite {v. (lookup p u * lookup q v when t = u + v) \<noteq> 0}" for t u
+  proof (rule finite_subset)
+    show "{v. (lookup p u * lookup q v when t = u + v) \<noteq> 0} \<subseteq> keys q"
+      by (rule, auto simp add: in_keys_iff simp del: lookup_not_eq_zero_eq_in_keys)
+  qed (fact finite_keys)
+  have "(\<Sum>t. monom_mult (lookup (p * q) t) 0 (subst_pp f t)) =
+        (\<Sum>t. \<Sum>u. monom_mult (lookup p u * (\<Sum>v. lookup q v when t = u + v)) 0 (subst_pp f t))"
+    by (simp add: times_poly_mapping.rep_eq prod_fun_def monom_mult_Sum_any[OF fin_1])
+  also have "\<dots> = (\<Sum>t. \<Sum>u. \<Sum>v. (monom_mult (lookup p u * lookup q v) 0 (subst_pp f t)) when t = u + v)"
+    by (simp add: Sum_any_right_distrib[OF fin_2] monom_mult_Sum_any[OF fin_3] mult_when when_monom_mult)
+  also have "\<dots> = (\<Sum>t. (\<Sum>(u, v). (monom_mult (lookup p u * lookup q v) 0 (subst_pp f t)) when t = u + v))"
+    apply (subst (2) Sum_any.cartesian_product [of "?P \<times> ?Q"])
+    apply (auto simp add: in_keys_iff monom_mult_left0 simp del: lookup_not_eq_zero_eq_in_keys)
+    done
+  also have "\<dots> = (\<Sum>(t, u, v). monom_mult (lookup p u * lookup q v) 0 (subst_pp f t) when t = u + v)"
+    apply (subst Sum_any.cartesian_product [of "?PQ \<times> (?P \<times> ?Q)"])
+    apply (auto simp add: fin_PQ in_keys_iff monom_mult_left0 simp del: lookup_not_eq_zero_eq_in_keys)
+    apply (metis monomial_0I mult_not_zero times_monomial_left)
+    done
+  also have "\<dots> = (\<Sum>(u, v, t). monom_mult (lookup p u * lookup q v) 0 (subst_pp f t) when t = u + v)"
+    using bij by (rule Sum_any.reindex_cong [of "\<lambda>(u, v, t). (t, u, v)"]) (simp add: fun_eq_iff)
+  also have "\<dots> = (\<Sum>(u, v). \<Sum>t. monom_mult (lookup p u * lookup q v) 0 (subst_pp f t) when t = u + v)"
+    apply (subst Sum_any.cartesian_product2 [of "(?P \<times> ?Q) \<times> ?PQ"])
+    apply (auto simp add: fin_PQ in_keys_iff monom_mult_left0 simp del: lookup_not_eq_zero_eq_in_keys)
+    apply (metis monomial_0I mult_not_zero times_monomial_left)
+    done
+  also have "\<dots> = (\<Sum>(u, v). monom_mult (lookup p u * lookup q v) 0 (subst_pp f u * subst_pp f v))"
+    by (simp add: subst_pp_plus)
+  also have "\<dots> = (\<Sum>u. \<Sum>v. monom_mult (lookup p u * lookup q v) 0 (subst_pp f u * subst_pp f v))"
+    apply (subst Sum_any.cartesian_product [of "?P \<times> ?Q"])
+    apply (auto simp add: in_keys_iff monom_mult_left0 simp del: lookup_not_eq_zero_eq_in_keys)
+    done
+  also have "\<dots> = (\<Sum>u. \<Sum>v. (monom_mult (lookup p u) 0 (subst_pp f u)) * (monom_mult (lookup q v) 0 (subst_pp f v)))"
+    by (simp add: times_monomial_left[symmetric] ac_simps mult_single)
+  also have "\<dots> = (\<Sum>t. monom_mult (lookup p t) 0 (subst_pp f t)) *
+                  (\<Sum>t. monom_mult (lookup q t) 0 (subst_pp f t))"
+    by (rule Sum_any_product [symmetric], (fact finite_monom_mult_lookup_not_zero)+)
+  finally show ?thesis by (simp add: poly_subst_alt)
+qed
+
+corollary poly_subst_monom_mult: "poly_subst f (monom_mult c t p) = monom_mult c 0 (subst_pp f t * poly_subst f p)"
+  by (simp only: times_monomial_left[symmetric] poly_subst_times poly_subst_monomial mult.assoc)
+
+corollary poly_subst_monom_mult': "poly_subst f (monom_mult c t p) = (monom_mult c 0 (subst_pp f t)) * poly_subst f p"
+  by (simp only: times_monomial_left[symmetric] poly_subst_times poly_subst_monomial)
+
+lemma poly_subst_sum: "poly_subst f (sum p A) = (\<Sum>a\<in>A. poly_subst f (p a))"
+  by (rule fun_sum_commute, simp_all add: poly_subst_plus)
+
+lemma poly_subst_prod: "poly_subst f (prod p A) = (\<Prod>a\<in>A. poly_subst f (p a))"
+  by (rule fun_prod_commute, simp_all add: poly_subst_times)
+
+lemma poly_subst_power: "poly_subst f (p ^ n) = (poly_subst f p) ^ n"
+  by (induct n, simp_all add: poly_subst_times)
+
+lemma poly_subst_id:
+  assumes "\<And>x. x \<in> indets p \<Longrightarrow> f x = monomial 1 (Poly_Mapping.single x 1)"
+  shows "poly_subst f p = p"
+proof -
+  have "poly_subst f p = (\<Sum>t\<in>keys p. monomial (lookup p t) t)"
+  proof (simp only: poly_subst_def, rule sum.cong, fact refl)
+    fix t
+    assume "t \<in> keys p"
+    have eq: "subst_pp f t = monomial 1 t"
+      by (rule subst_pp_id, rule assms, erule in_indetsI, fact \<open>t \<in> keys p\<close>)
+    show "monom_mult (lookup p t) 0 (subst_pp f t) = monomial (lookup p t) t"
+      by (simp add: eq monom_mult_monomial)
+  qed
+  also have "... = p" by (simp only: poly_mapping_sum_monomials)
+  finally show ?thesis .
+qed
+
+lemma in_indets_poly_substE:
+  assumes "x \<in> indets (poly_subst f p)"
+  obtains y where "y \<in> indets p" and "x \<in> indets (f y)"
+proof -
+  note assms
+  also have "indets (poly_subst f p) \<subseteq> (\<Union>t\<in>keys p. indets (monom_mult (lookup p t) 0 (subst_pp f t)))"
+    unfolding poly_subst_def by (rule indets_sum_subset)
+  finally obtain t where "t \<in> keys p" and "x \<in> indets (monom_mult (lookup p t) 0 (subst_pp f t))" ..
+  note this(2)
+  also have "indets (monom_mult (lookup p t) 0 (subst_pp f t)) \<subseteq> keys (0::('a \<Rightarrow>\<^sub>0 nat)) \<union> indets (subst_pp f t)"
+    by (rule indets_monom_mult_subset)
+  also have "... = indets (subst_pp f t)" by simp
+  finally obtain y where "y \<in> keys t" and "x \<in> indets (f y)" by (rule in_indets_subst_ppE)
+  from this(1) \<open>t \<in> keys p\<close> have "y \<in> indets p" by (rule in_indetsI)
+  from this \<open>x \<in> indets (f y)\<close> show ?thesis ..
+qed
+
+lemma poly_deg_poly_subst_eq_zeroI:
+  assumes "\<And>x. x \<in> indets p \<Longrightarrow> poly_deg (f x) = 0"
+  shows "poly_deg (poly_subst f (p::('n \<Rightarrow>\<^sub>0 nat) \<Rightarrow>\<^sub>0 'b::comm_semiring_1)) = 0"
+proof (cases "p = 0")
+  case True
+  thus ?thesis by simp
+next
+  case False
+  have "poly_deg (poly_subst f p) \<le> Max (poly_deg ` (\<lambda>t. monom_mult (lookup p t) 0 (subst_pp f t)) ` keys p)"
+    unfolding poly_subst_def by (fact poly_deg_sum_le)
+  also have "... \<le> 0"
+  proof (rule Max.boundedI)
+    show "finite (poly_deg ` (\<lambda>t. monom_mult (lookup p t) 0 (subst_pp f t)) ` keys p)"
+      by (simp add: finite_image_iff)
+  next
+    from False show "poly_deg ` (\<lambda>t. monom_mult (lookup p t) 0 (subst_pp f t)) ` keys p \<noteq> {}" by simp
+  next
+    fix d
+    assume "d \<in> poly_deg ` (\<lambda>t. monom_mult (lookup p t) 0 (subst_pp f t)) ` keys p"
+    then obtain t where "t \<in> keys p" and d: "d = poly_deg (monom_mult (lookup p t) 0 (subst_pp f t))"
+      by fastforce
+    have "d \<le> deg_pm (0::'n \<Rightarrow>\<^sub>0 nat) + poly_deg (subst_pp f t)"
+      unfolding d by (fact poly_deg_monom_mult_le)
+    also have "... = poly_deg (subst_pp f t)" by simp
+    also have "... = 0" by (rule poly_deg_subst_pp_eq_zeroI, rule assms, erule in_indetsI, fact)
+    finally show "d \<le> 0" .
+  qed
+  finally show ?thesis by simp
+qed
+
+lemma poly_deg_poly_subst_le:
+  assumes "\<And>x. x \<in> indets p \<Longrightarrow> poly_deg (f x) \<le> 1"
+  shows "poly_deg (poly_subst f (p::('n \<Rightarrow>\<^sub>0 nat) \<Rightarrow>\<^sub>0 'b::comm_semiring_1)) \<le> poly_deg p"
+proof (cases "p = 0")
+  case True
+  thus ?thesis by simp
+next
+  case False
+  have "poly_deg (poly_subst f p) \<le> Max (poly_deg ` (\<lambda>t. monom_mult (lookup p t) 0 (subst_pp f t)) ` keys p)"
+    unfolding poly_subst_def by (fact poly_deg_sum_le)
+  also have "... \<le> poly_deg p"
+  proof (rule Max.boundedI)
+    show "finite (poly_deg ` (\<lambda>t. monom_mult (lookup p t) 0 (subst_pp f t)) ` keys p)"
+      by (simp add: finite_image_iff)
+  next
+    from False show "poly_deg ` (\<lambda>t. monom_mult (lookup p t) 0 (subst_pp f t)) ` keys p \<noteq> {}" by simp
+  next
+    fix d
+    assume "d \<in> poly_deg ` (\<lambda>t. monom_mult (lookup p t) 0 (subst_pp f t)) ` keys p"
+    then obtain t where "t \<in> keys p" and d: "d = poly_deg (monom_mult (lookup p t) 0 (subst_pp f t))"
+      by fastforce
+    have "d \<le> deg_pm (0::'n \<Rightarrow>\<^sub>0 nat) + poly_deg (subst_pp f t)"
+      unfolding d by (fact poly_deg_monom_mult_le)
+    also have "... = poly_deg (subst_pp f t)" by simp
+    also have "... \<le> deg_pm t" by (rule poly_deg_subst_pp_le, rule assms, erule in_indetsI, fact)
+    also from \<open>t \<in> keys p\<close> have "... \<le> poly_deg p" by (rule poly_deg_max_keys)
+    finally show "d \<le> poly_deg p" .
+  qed
+  finally show ?thesis by simp
+qed
+
+subsection \<open>Locale @{term pm_powerprod}\<close>
+
+locale pm_powerprod =
+  ordered_powerprod ord ord_strict
+  for ord::"('n::countable \<Rightarrow>\<^sub>0 nat) \<Rightarrow> ('n \<Rightarrow>\<^sub>0 nat) \<Rightarrow> bool" (infixl "\<preceq>" 50)
+  and ord_strict (infixl "\<prec>" 50)
+begin
+
+sublocale gd_powerprod ..
+
+end
+
+end (* theory *)
